\section{Building the equation of motion}
Let us consider a scalar field with zero conformal weight that is, under an infinitesimal conformal transformation
\begin{equation}
  \d_\omega g_{\m\n }=2\omega g_{\m\n },\qquad \d_\omega\f=0
\end{equation}

Let us consider the most general second-order pseudoscalar constructed from the scalar field $\f$ and its derivatives up to second order, together with the metric tensor and its associates curvature
\begin{equation}
	\E =\sqrt{-g}E\left(\f,\nabla_\m \f ,\nabla_\m \nabla_\n \f ,g_{\m\n },R_{\m\n }^{\a\b }\right)=0
\end{equation}
The variation of this equation under infinitesimal conformal transformations reads,
\begin{align}
  \d_\omega \E&=\d_\omega(\sqrt{-g})E+\sqrt{-g}\d_\omega E\\
  &=-\frac{1}{2}\sqrt{-g}g_{\m\n }\d_\omega g^{\m\n }E+\sqrt{-g}\d_\omega E
\end{align}
From $\d_\omega g_{\m\n }=2\omega g_{\m\n }$ and $\d_\omega(g_{\m\n }g^{\m\n })=0$ implies that
\begin{equation}
  g_{\m\n }\d_\omega g^{\m\n }=-g^{\m\n }\d_\omega g_{\m\n }
\end{equation}
Furthermore, from \eqref{delta-nabla} and \eqref{delta-nabla-nabla}, we have
\begin{align}
  \d_\omega \E&=\pdv{E}{\f }\cancelto{0}{\d_\omega \f} +\pdv{E}{(\nabla_\m \f )}\cancelto{0}{\d_\omega \nabla_\m \f} +\pdv{E}{(\nabla_\m \nabla_\n \f )}\d_\omega (\nabla_\m \nabla_\n \f )+\pdv{E}{g^{\m\n }}\d_\omega g^{\m\n }+P^{\m\n }_{\a\b }\d_\omega R^{\a\b }_{\m\n }
\end{align}
where we have defined 
\begin{equation}\label{P-trnsor}
  P^{\m\n }_{\a\b }:=\pdv{E}{R_{\m\n }^{\a\b }},\qquad   P^\m_\n :=P^{\a\m }_{\a\n }
\end{equation}

So then
\begin{align*}
  \d_\omega \E&=-\frac{1}{2}\sqrt{-g}g_{\m\n }\d_\omega g^{\m\n }E+\sqrt{-g}\pdv{E}{(\nabla_\m \nabla_\n \f  )}\d_\omega (\nabla_\m \nabla_\n \f )+\sqrt{-g}\pdv{E}{g^{\m\n }}\d_\omega g^{\m\n }+\sqrt{-g}P^{\m\n }_{\a\b }\d_\omega R^{\a\b }_{\m\n }\\
  &=\sqrt{-g}\pdv{E}{(\nabla_\m \nabla_\n \f )}\left(g_{\n\b }\nabla^\r \f\nabla_\r\omega-2\nabla_{(\m }\f\nabla_{\n)}\omega\right)+\sqrt{-g}\pdv{E}{g^{\m\n }}\d_\omega g^{\m\n }+\sqrt{-g}P^{\m\n }_{\a\b }\d_\omega R^{\a\b }_{\m\n }\\& -\frac{1}{2}\sqrt{-g}g_{\m\n }\d_\omega g^{\m\n }E\\
  &=\sqrt{-g}\pdv{E}{(\nabla_\m \nabla_\n \f )}\left(g_{\n\b }\nabla^\r \f\nabla_\r\omega-2\nabla_{(\m }\f\nabla_{\n)}\omega\right)+\sqrt{-g}P^{\m\n }_{\a\b }\d_\omega R^{\a\b }_{\m\n }-2\omega g^{\m\n}\sqrt{-g}\left(\pdv{E}{g^{\m\n }}-\frac{1}{2}g_{\m\n }E\right)
\end{align*}
Note that
\begin{align}
  \pdv{(\sqrt{-g}E)}{g^{\m\n }}&=-\frac{1}{2}\sqrt{-g}g_{\m\n }E+\sqrt{-g}\pdv{E}{g^{\m\n }}\\
  &=\sqrt{-g}\left(\pdv{E}{g^{\m\n }}-\frac{1}{2}g_{\m\n }E\right) \label{d-sqrt-E}
\end{align}
By defining
\begin{align}\label{A-B}
  A^{\m\n }:=\pdv{E}{(\nabla_\m \nabla_\n\f )},\qquad B_{\m\n }=-2\left(\pdv{E}{g^{\m\n }}-\frac{1}{2}g_{\m\n }E\right)=-\frac{2}{\sqrt{-g}}\pdv{(\sqrt{-g}E)}{g^{\m\n }}
\end{align}
we obtain
\begin{align}
  \d_\omega \E&=\sqrt{-g}A^{\m\n }\left(g_{\m\n }\nabla^\r \f \nabla_\r \omega-2\nabla_\m \f\nabla_\n \omega\right)+\sqrt{-g}P^{\m\n }\d_\omega R^{\a\b }_{\m\n }+\sqrt{-g}\omega B_{\m\n }g_{\m\n }\\
  &=\sqrt{-g}\left(A\nabla^\r \f\nabla_\r \omega-2A^{\m\n}\nabla_\m \f\nabla_\n\omega+\omega B+P^{\m\n}_{\a\b}\d_\omega R^{\a\b }_{\m\n }\right)
\end{align}
Using
\begin{equation}
  \d_\omega R^\a _{~\b\m\n }=2\nabla_{[\m }\d_\omega \G^\a _{~\n]\b }
\end{equation}
we have
\begin{align}
    \d_\omega \E&=\sqrt{-g}\left(A\nabla^\r \f\nabla_\r \omega-2A^{\m\n}\nabla_\m \f\nabla_\n\omega+\omega B+2P_\a ^{~\b\m\n }\nabla_{[\m }\d_\omega \G^{\a }_{~\n]\b }\right)\\
    &=\sqrt{-g}\left(A\nabla^\n \f\nabla_\n  \omega-2A^{\m\n}\nabla_\m \f\nabla_\n\omega+\omega B+2P_\a ^{~\b\m\n }\nabla_{[\m }\d_\omega \G^{\a }_{~\n]\b }\right)\\
    &=\sqrt{-g}\left[(A\nabla^\n \f -2A^{\m\n }\nabla_\m\f )\nabla_\n \omega+\omega B+2P_\a ^{~\b\m\n }\nabla_{[\m }\d_\omega \G^{\a }_{~\n]\b }\right]
\end{align}

Noting that
\begin{align}
  \d_\omega \G^\a_{~\n\b }&=\frac{1}{2}g^{\a\lambda}\left[\nabla_\n (\d_\omega g_{\b\lambda})+\nabla_\b (\d_\omega g_{\n\lambda})-\nabla_\lambda(\d_\omega g_{\n\b })\right]\\
  &=g^{\a\lambda}\left(g_{\b\lambda}\nabla_\n\omega +g_{\n\lambda}\nabla_\b\omega-g_{\n\b }\nabla_\lambda\omega\right)\\
  &=g^{\a\lambda}\left(g_{\b\lambda}\nabla_\n\omega +2g_{\n[\lambda}\nabla_{\b]}\omega\right)
\end{align}
we obtain
\begin{align*}
  \d_\omega\E&=\sqrt{-g}\left[(A\nabla^\n \f -2A^{\m\n }\nabla_\m\f )\nabla_\n \omega+\omega B+2P_\a ^{~\b\m\n }\nabla_{\m }g^{\a\lambda}\left(g_{\b\lambda}\nabla_\n\omega +2g_{\n[\lambda}\nabla_{\b]}\omega\right)\right]\\
  &=\sqrt{-g}\left[(A\nabla^\n \f -2A^{\m\n }\nabla_\m\f )\nabla_\n \omega+\omega B+2P ^{\lambda\b\m\n }\nabla_{\m }\left(\cancel{g_{\b\lambda}}\nabla_\n\omega +2g_{\n\lambda}\nabla_{\b}\omega\right)\right]\\
  &=\sqrt{-g}\left[(A\nabla^\n \f -2A^{\m\n }\nabla_\m\f )\nabla_\n \omega+\omega B+4P^{\lambda\b\m\n }\nabla_{\m }g_{\n\lambda}\nabla_{\b}\omega\right]\\
  &=\sqrt{-g}\left[(A\nabla^\n \f -2A^{\m\n }\nabla_\m\f )\nabla_\n \omega+\omega B-4P^{\m\n }\nabla_{\m }\nabla_{\n }\omega\right]
\end{align*}
Imposing $\d_\omega\E=0$ for all $\omega$, we obtain the following conditions,
\begin{subequations}\label{conditions}
	\begin{align}
 \label{A-condition} A\nabla^\n \f-2A^{\m\n }\nabla_\m \f&=0\\
  \label{B-condition} B&=0\\
 \label{P-condition} P^{\m\n }&=0
\end{align}
\end{subequations}
 
From \eqref{P-tensor},
\begin{equation}\label{dEdP}
    \pdv{E}{R^{\m\n }_{\a\b }}= P^{\alpha\beta}_{\mu\nu}=\hat{H}^{\alpha\beta}_{\mu\nu}+\delta^{[\alpha}_{[\mu}\hat{I}^{\beta]}_{\nu]}+J\delta^\alpha_{[\mu}\delta^\beta_{\nu]}
\end{equation}
we notice that since $\hat{H}^{\alpha\beta}_{\mu\nu}$ is the traceless part of $H^{\alpha\beta}_{\mu\nu}$,
\begin{equation}
  P^\b_\n =P^{\a\b }_{\a\n }=\delta^{[\alpha}_{[\a }\hat{I}^{\beta]}_{\nu]}+J\delta^\alpha_{[\a }\delta^\beta_{\nu]}
\end{equation}

Since the variation with respect to the Weyl tensor does not contribute to the first trace \eqref{dEdP}, the contribution of the Riemann tensor to $E$ has to be through its traceless part,
\begin{equation}
	\E =\sqrt{-g}E\left(\f,\nabla_\m \f ,\nabla_\m \nabla_\n \f ,g_{\m\n },C_{\m\n }^{\a\b }\right)=0\,.
\end{equation}

\begin{ej}
	Let us consider the following action principle
	\begin{align}
  S[\f,g]&=\int\dd^Dx\sqrt{-g}\left(-\frac{1}{2}\nabla_\m \f\nabla^\m \f \right)^{D/2}\\
  &=\int\dd^Dx\sqrt{-g}\left(-\frac{1}{2}(\nabla\f )^2\right)^{D/2}\\
  &=\int\dd^Dx\sqrt{-g}X^{D/2}
\end{align}
where we have defined $X:=-\frac{1}{2}\nabla_\m \f\nabla^\m \f$. 

Now, we must to find $E$. Varying with respect to $\f$,
\begin{align}
  \d_\f S&=-\int\dd^Dx\sqrt{-g}\frac{D}{2}\left(-\frac{1}{2}(\nabla\f )^2\right)^{\frac{D-2}{2}}\nabla^\m\f \nabla_\m \d\f \\
  &=\int\dd^Dx\sqrt{-g}\frac{D}{2}\nabla_\m \left[\left(-\frac{1}{2}(\nabla\f )^2\right)^{\frac{D-2}{2}}\nabla^\m \f \right]\d\f +\rm b.t
\end{align}
therefore,
\begin{align}
  E&=\nabla_\m \left[\left(-\frac{1}{2}(\nabla\f )^2\right)^{\frac{D-2}{2}}\nabla^\m \f \right]\\
  &=\frac{D-2}{2}\left(-\frac{1}{2}(\nabla\f )^2\right)^{\frac{D-4}{2}}(-1)\nabla^\a \f \nabla_\m \nabla_\a\f \nabla^\m \f +\left(-\frac{1}{2}(\nabla\f )^2\right)^{\frac{D-2}{2}}\Box\f 
\end{align}
which can be rewritten as
\begin{equation}
  E=X^{\frac{D-2}{2}}\Box\f -\frac{D-2}{2}X^{\frac{D-4}{2}}\nabla_\m \nabla_\n \f\nabla^\m \f\nabla^\n \f 
\end{equation}

Let's see how \eqref{A-condition} looks,
\begin{align}
  A^{\m\n }&=\pdv{(\nabla_\m \f\nabla_\n \f  )}\left[X^{\frac{D-2}{2}}g^{\m\n }\nabla_\m\f \nabla_\n\f  -\frac{D-2}{2}X^{\frac{D-4}{2}}\nabla_\m \nabla_\n \f\nabla^\m \f\nabla^\n \f \right]\\
  &=X^{\frac{D-2}{2}}g^{\m\n }-\frac{D-2}{2}X^{\frac{D-4}{2}}\nabla^\m \f \nabla^\n\f 
\end{align}
and its trace yields
\begin{align}
  A&=DX^{\frac{D-2}{2}}-\frac{D-2}{2}X^{\frac{D-4}{2}}(\nabla\f )^2\\
  &=DX^{\frac{D-2}{2}}+(D-2)X^{\frac{D-4}{2}}\left(-\frac{1}{2}(\nabla\f )^2\right)\\
  &=DX^{\frac{D-2}{2}}+(D-2)X^{\frac{D-2}{2}}\\
  &=2(D-1)X^{\frac{D-2}{2}}
\end{align}
Pluggin into \eqref{A-condition},
\begin{align*}
  A\nabla^\n \f-2A^{\m\n }\nabla_\m \f&=2(D-1)X^{\frac{D-2}{2}}\nabla^\n\f -2X^{\frac{D-2}{2}}g^{\m\n }\nabla_\m \f +(D-2)X^{\frac{D-4}{2}}\nabla^\m\f \nabla^\n\f \nabla_\m\f \\
  &=2(D-1)X^{\frac{D-2}{2}}\nabla^\n\f-2X^{\frac{D-2}{2}}\nabla^\n\f +(D-2)X^{\frac{D-4}{2}}(\nabla\f )^2\nabla^\n\f \\
  &=\left[2(D-2)X^{\frac{D-2}{2}}-2(D-2)X^{\frac{D-4}{2}}X\right]\nabla^\n\f \\
  &=\left[2(D-2)X^{\frac{D-2}{2}}-2(D-2)X^{\frac{D-2}{2}}2\right]\nabla^\n\f \\
  &=0\qquad \checkmark
\end{align*}
\end{ej}

%--------------------


We notice that the constraints \eqref{conditions} on $E$ are an overdetermined linear PDE system with the following characteristic vector fields
\begin{align}
	Z&=g^{\m\n }\pdv{g^{\m\n }}-\frac{D}{2}E\pdv{E},\\
	Z^\n &=\left(g_{\a\m }g^{\b\n }\nabla_\b \f -2\d^\n_\a \nabla_\m \f \right)\pdv{(\nabla_\a\nabla_\m \f )}
\end{align}
Let's see the integrability of the system. To do that, we compute the commutators between the vector fields. It is straightforward to see that $[Z^\n, Z^\lambda ]=0$. On the other hand
\begin{align}
  [Z,Z^\n ]&=ZZ^\n -\cancel{Z^\n  Z}\\
  &=\left[\left(g^{\r\t }\pdv{g^{\r\t }}-\frac{DE}{2}\pdv{E}\right),(g_{\a\m }g^{\b\n }\f_\b -2\d^\n_\a \f_\m )\pdv{\f_{\a\m }}\right]\\
  &=g^{\r\t }\pdv{g^{\r\t }}(g_{\a\m }g^{\b\n })\f_\b\pdv{\f_{\a\m }}
\end{align}
For compute the derivative, we note that
\begin{equation}
  \d (g_{\a\m }g^{\b\n })=g^{\b\n }\d g_{\a\m }+g_{\a\m }\d g^{\b\n }.
\end{equation}
Using that
\begin{equation}
  \d g_{\a\m }=-g_{\a\r }g_{\m\t }\d g^{\r\t },
\end{equation}
we obtain
\begin{equation}
  \d (g_{\a\m }g^{\b\n })=-g^{\b\n }g_{\a\r }g_{\m\t }\d g^{\r\t }+g_{\a\m }\d^\b_\r \d^\n_\t \d g^{\r\t }.
\end{equation}
Moreover,
\begin{equation}
  \d (g_{\a\m }g^{\b\n })=\pdv{g^{\r\t }}(g_{\a\m }g^{\b\n })\d g^{\r\t },
\end{equation}
which implies that
\begin{equation}
  \pdv{g^{\r\t }}(g_{\a\m }g^{\b\n })=-g^{\b\n }g_{\a(\r }g_{\m|\t) }+g_{\a\m }\d^\b_{(\r} \d^\n_{\t)}.
\end{equation}
Finally,
\begin{align}
  [Z,Z^\n ]&=g^{\r\t }\pdv{g^{\r\t }}(g_{\a\m }g^{\b\n })\f_\b\pdv{\f_{\a\m }}\\
  &=g^{\r\t }(g_{\a\m }\d^\b_\r \d^\n_\t -g^{\b\n }g_{\a\r }g_{\m\t })\f_\b \pdv{\f_{\a\m }}\\
  &=(g^{\b\n }g_{\a\m }-g^{\b\n }\d^\t_\a g_{\m\t })\f_\b \pdv{\f_{\a\m }}\\
  &=(g^{\b\n }g_{\a\m }-g^{\b\n }g_{\a\m })\f_\b \pdv{\f_{\a\m }}\\
  &=0.
\end{align}
Then, the system is integrable.

The characteristic system of $Z$ is
\begin{equation}
  \frac{\dd g^{11}}{g^{11}}=\cdots=\frac{\dd g^{\a\b }}{g^{\a\b }}=\cdots=\frac{\dd g^{DD}}{g^{DD}}=\frac{\dd E}{\frac{DE}{2}}.
\end{equation}
For $\a,\b $ fixed, a combination of the characteristic equations can also be incorporated, giving
\begin{equation}
  \frac{\dd g^{\a\b }}{g^{\a\b }}=\frac{C_{\m\n }\dd g^{\m\n }}{C_{\m\n }g^{\m\n }}\implies \dd (\ln g^{\a\b })=\dd(\ln C_{\m\n }g^{\m\n }),
\end{equation}
where $C_{\m\n }$ is an arbitrary tensor which does not depend on $g_{\m\n }$. By integrating and exponentiating both sides, we obtain the invariant
\begin{equation}
  \Omega^{\a\b }=\frac{g^{\a\b }}{C_{\m\n }g^{\m\n }}.
\end{equation}
Choosing $C_{\m\n }=-\frac{1}{2}\f_\m \f_\n $ we recover the auxilliary metric
\begin{equation}
  \Omega^{\a\b }=\frac{g^{\a\b }}{X}=\tilde{g}^{\a\b }.
\end{equation}
They corresponds to $\frac{D(D+1)}{2}-1$ invariants, since their symmetry and the condition $C_{\m\n }\Omega^{\m\n }=1$. The general solution to $Z(E)=0$ can be obtained from
\begin{equation}
  \frac{\dd X}{X}=\frac{\dd E}{\frac{DE}{2}}\implies \ln X=\frac{2}{D}\ln E,
\end{equation}
giving
\begin{equation}
  E=X^\frac{D}{2}\tilde{E}(\f,\f_\m ,\f_{\m\n },\tilde{g}^{\m\n },\tilde{C}^{\a\b }_{\m\n }).
\end{equation}
Now, we have to find the general solution to $Z^\n (E)=0$. First, we notice that
\begin{align}
  \tilde{\f}_{\m\n }&:=\tilde{\nabla}_\m \tilde{\nabla}_\n \f \\
  &=\partial_\m \partial_\n \f -\tilde{\G }^\a _{~\m\n }\partial_\a\f
\end{align}

















































































